Add interpreter for signature

doc/coq/signature/Concrete.v
@@ -134,3 +134,859 @@ Notation "'{|' ll '~>' rr '|}'" :=
 Notation "'{|' ll '~>*' rr '|}'" := 
   (multi_step ll rr) 
   (at level 10, ll at next level, rr at next level).
+
+Inductive interpreter_state `{time T} :=
+  | Pending (reached : list (config T))
+  | Error (reached : list (config T)) (* Type error *)
+  | Resolved (V : @dy_value T) (m : @memory T) (t : T) (reached : list (@config T))
+.
+
+Fixpoint eval `{time T} e C m t (reached : list (@config T)) (FUEL : nat) :=
+  let reached := (Cf e C m t) :: reached in
+  match FUEL with
+  | 0 => Pending reached
+  | S FUEL' =>
+    match e with
+    | e_var x =>
+      match addr_x C x with
+      | None => Error reached
+      | Some addr =>
+        match read m addr with
+        | None => Error reached
+        | Some v => Resolved (EVal v) m t ((Rs (EVal v) m t) :: reached)
+        end
+      end
+    | e_lam x e =>
+      let v := Fun x e C in
+      Resolved (EVal v) m t ((Rs (EVal v) m t) :: reached)
+    | e_app e1 e2 =>
+      match eval e1 C m t reached FUEL' with
+      | Resolved (EVal (Fun x e C_f)) m_f t_f reached' =>
+        match eval e2 C m_f t_f reached' FUEL' with
+        | Resolved (EVal v) m_a t_a reached'' =>
+          match eval e (dy_binde x (tick C m_a t_a x v) C_f) ((tick C m_a t_a x v) !-> v; m_a) (tick C m_a t_a x v) reached'' FUEL' with
+          | Resolved (EVal v') m' t' reached''' => Resolved (EVal v') m' t' reached'''
+          | Resolved _ _ _ reached''' => Error reached'''
+          | other => other
+          end
+        | Resolved _ _ _ reached'' => Error reached''
+        | other => other
+        end
+      | Resolved (EVal (Func M s_M e C_f)) m_f t_f reached' =>
+        match eval e2 C m_f t_f reached' FUEL' with
+        | Resolved (MVal C_v) m_a t_a reached'' =>
+          match project C_v s_M with
+          | None => Error reached''
+          | Some C_M =>
+          match eval e (dy_bindm M C_M C_f) m_a t_a reached'' FUEL' with
+          | Resolved (EVal v') m' t' reached''' => Resolved (EVal v') m' t' reached'''
+          | Resolved _ _ _ reached''' => Error reached'''
+          | other => other
+          end end
+        | Resolved _ _ _ reached'' => Error reached''
+        | other => other
+        end
+      | Resolved _ _ _ reached' => Error reached'
+      | other => other
+      end
+    | e_link e1 e2 =>
+      match eval e1 C m t reached FUEL' with
+      | Resolved (MVal C') m' t' reached' =>
+        match eval e2 C' m' t' reached' FUEL' with
+        | Resolved V m'' t'' reached'' => Resolved V m'' t'' reached''
+        | other => other
+        end
+      | Resolved _ _ _ reached' => Error reached'
+      | other => other
+      end
+    | m_empty => Resolved (MVal C) m t ((Rs (MVal C) m t) :: reached)
+    | m_var M =>
+      match ctx_M C M with
+      | None => Error reached
+      | Some C_M => Resolved (MVal (C_M[|C|])) m t ((Rs (MVal (C_M[|C|])) m t) :: reached)
+      end
+    | m_lam M s e =>
+      let v := Func M s e C in
+      Resolved (EVal v) m t ((Rs (EVal v) m t) :: reached)
+    | m_app e1 e2 s =>
+      match eval e1 C m t reached FUEL' with
+      | Resolved (EVal (Fun x e C_f)) m_f t_f reached' =>
+        match eval e2 C m_f t_f reached' FUEL' with
+        | Resolved (EVal v) m_a t_a reached'' =>
+          match eval e (dy_binde x (tick C m_a t_a x v) C_f) ((tick C m_a t_a x v) !-> v; m_a) (tick C m_a t_a x v) reached'' FUEL' with
+          | Resolved (MVal C') m' t' reached''' =>
+            match project C' s with
+            | Some C'' => Resolved (MVal (C''[|C|])) m' t' 
+              ((Rs (MVal (C''[|C|])) m' t') :: reached''')
+            | None => Error reached'''
+            end
+          | Resolved _ _ _ reached''' => Error reached'''
+          | other => other
+          end
+        | Resolved _ _ _ reached'' => Error reached''
+        | other => other
+        end
+      | Resolved (EVal (Func M s_M e C_f)) m_f t_f reached' =>
+        match eval e2 C m_f t_f reached' FUEL' with
+        | Resolved (MVal C_v) m_a t_a reached'' =>
+          match project C_v s_M with
+          | None => Error reached''
+          | Some C_M =>
+          match eval e (dy_bindm M C_M C_f) m_a t_a reached'' FUEL' with
+          | Resolved (MVal C') m' t' reached''' => 
+            match project C' s with
+            | Some C'' => Resolved (MVal (C''[|C|])) m' t'
+              ((Rs (MVal (C''[|C|])) m' t') :: reached''')
+            | None => Error reached'''
+            end
+          | Resolved _ _ _ reached''' => Error reached'''
+          | other => other
+          end end
+        | Resolved _ _ _ reached'' => Error reached''
+        | other => other
+        end
+      | Resolved _ _ _ reached' => Error reached'
+      | other => other
+      end
+    end
+  end.
+
+Ltac rep_eval SOLVER :=
+  match goal with
+  | |- context [match project ?C ?s with _ => _ end] =>
+    let PROJ := fresh "PROJ" in
+    destruct (project C s) eqn:PROJ; clarify;
+    rep_eval SOLVER
+  | [RR : eval ?e ?C ?m ?t ?l ?n = _ |- 
+          context [eval ?e ?C ?m ?t ?l ?n]] =>
+    (* trivial case *)
+    rewrite RR;
+    move RR at top
+  | [RR : eval ?e ?C ?m ?t ?l ?n = _ |-
+      context [eval ?e ?C ?m ?t ?l ?n0]] =>
+    (* relaxation *)
+    replace (eval e C m t l n0) with (eval e C m t l n);
+    rewrite RR;
+    (* IHFUEL *)
+    try (symmetry; apply SOLVER; eauto; fail);
+    (* relax_fuel *)
+    try (symmetry; apply SOLVER with (FUEL := n); try nia; eauto; fail);
+    move RR at top
+  | [RR : eval ?e ?C ?m ?t ?l ?n = _ |-
+      context [eval ?e ?C ?m ?t ?l0 ?n0]] =>
+    (* relaxation, l is an evar *)
+    replace (eval e C m t l0 n0) with (eval e C m t l n);
+    rewrite RR;
+    (* IHFUEL *)
+    try (symmetry; apply SOLVER; eauto; fail);
+    (* relax_fuel *)
+    try (symmetry; apply SOLVER with (FUEL := n); try nia; eauto; fail);
+    move RR at top
+  end.
+
+Lemma relax_fuel `{time T} :
+  forall FUEL FUEL' (LE : FUEL <= FUEL') e C m t l l' V m' t'
+    (EVAL : eval e C m t l FUEL = Resolved V m' t' l'),
+    eval e C m t l FUEL' = Resolved V m' t' l'.
+Proof.
+  rename H into ET. rename H0 into OT. rename H1 into TT.
+  induction FUEL; intros.
+  - inversion EVAL.
+  - inversion LE; eauto. 
+    assert (FUEL <= m0) as HINT. { nia. }
+    specialize (IHFUEL m0 HINT).
+    destruct e; simpl in *; eauto; repeat des_hyp;
+    rep_eval IHFUEL;
+    rep_eval IHFUEL; eauto;
+    rep_eval IHFUEL; eauto.
+    all:rep_eval IHFUEL.
+Qed.
+
+Lemma relax_fuel_err `{time T} :
+  forall FUEL FUEL' (LE : FUEL <= FUEL') e C m t l l'
+    (EVAL : eval e C m t l FUEL = Error l'),
+    eval e C m t l FUEL' = Error l'.
+Proof.
+  rename H into ET. rename H0 into OT. rename H1 into TT.
+  induction FUEL; intros.
+  inversion EVAL.
+  inversion LE; eauto. 
+  assert (FUEL <= m0) as HINT. { nia. }
+  specialize (IHFUEL m0 HINT).
+  destruct e; simpl in *; eauto; repeat des_hyp;
+  try (erewrite IHFUEL; eauto; fail);
+  try (erewrite relax_fuel; eauto);
+  simpl; eauto;
+  try solve 
+    [do 3 (rep_eval IHFUEL; eauto) |
+     do 3 (rep_eval relax_fuel; eauto)].
+  all: rep_eval relax_fuel; rep_eval IHFUEL; eauto.
+Qed.
+
+Lemma Eval_well_defined_l :
+  forall `{time T} e (C : @dy_ctx T) m t V m' t' 
+    (R : {| Cf e C m t ~> Rs V m' t' |}) l,
+    exists FUEL, 
+      match eval e C m t l FUEL with
+      | Resolved V' m'' t'' _ => V = V' /\ m' = m'' /\ t' = t''
+      | _ => False
+      end.
+Proof.
+  intros. revert l. remember (Cf e C m t) as cf. remember (Rs V m' t') as rs.
+  generalize dependent e. generalize dependent V. revert C m t m' t'.
+  induction R; intros; inversion Heqcf; inversion Heqrs; subst.
+  - exists 1; simpl. rewrite ADDR. rewrite ACCESS. eauto.
+  - exists 1; simpl; eauto.
+  - edestruct IHR1 as [FUEL' EQ']; eauto. clear IHR1. des_hyp.
+    edestruct IHR2 as [FUEL'' EQ'']; eauto. clear IHR2. des_hyp.
+    edestruct IHR3 as [FUEL''' EQ''']; eauto. clear IHR3. des_hyp.
+    exists (S (Nat.max FUEL' (Nat.max FUEL'' FUEL'''))).
+    simpl.
+    destruct EQ' as [? [? ?]]. subst.
+    destruct EQ'' as [? [? ?]]. subst.
+    destruct EQ''' as [? [? ?]]. subst.
+    rep_eval relax_fuel.
+    rep_eval relax_fuel.
+    rep_eval relax_fuel. eauto.
+  - edestruct IHR1 as [FUEL' EQ']; eauto. clear IHR1. des_hyp.
+    edestruct IHR2 as [FUEL'' EQ'']; eauto. clear IHR2. des_hyp.
+    edestruct IHR3 as [FUEL''' EQ''']; eauto. clear IHR3. des_hyp.
+    exists (S (Nat.max FUEL' (Nat.max FUEL'' FUEL'''))).
+    simpl.
+    destruct EQ' as [? [? ?]]. subst.
+    destruct EQ'' as [? [? ?]]. subst.
+    destruct EQ''' as [? [? ?]]. subst.
+    rep_eval relax_fuel.
+    rep_eval relax_fuel.
+    rep_eval relax_fuel. eauto.
+  - edestruct IHR1 as [FUEL' EQ']; eauto. clear IHR1. des_hyp.
+    edestruct IHR2 as [FUEL'' EQ'']; eauto. clear IHR2. des_hyp.
+    exists (S (Nat.max FUEL' FUEL'')).
+    simpl.
+    destruct EQ' as [? [? ?]]. subst.
+    destruct EQ'' as [? [? ?]]. subst.
+    rep_eval relax_fuel.
+    rep_eval relax_fuel. eauto.
+  - exists 1. simpl; eauto.
+  - exists 1; simpl. rewrite ACCESS. eauto.
+  - exists 1; simpl; eauto.
+  - edestruct IHR1 as [FUEL' EQ']; eauto. clear IHR1. des_hyp.
+    edestruct IHR2 as [FUEL'' EQ'']; eauto. clear IHR2. des_hyp.
+    edestruct IHR3 as [FUEL''' EQ''']; eauto. clear IHR3. des_hyp.
+    exists (S (Nat.max FUEL' (Nat.max FUEL'' FUEL'''))).
+    simpl.
+    destruct EQ' as [? [? ?]]. subst.
+    destruct EQ'' as [? [? ?]]. subst.
+    destruct EQ''' as [? [? ?]]. subst.
+    do 4 rep_eval relax_fuel.
+  - edestruct IHR1 as [FUEL' EQ']; eauto. clear IHR1. des_hyp.
+    edestruct IHR2 as [FUEL'' EQ'']; eauto. clear IHR2. des_hyp.
+    edestruct IHR3 as [FUEL''' EQ''']; eauto. clear IHR3. des_hyp.
+    exists (S (Nat.max FUEL' (Nat.max FUEL'' FUEL'''))).
+    simpl.
+    destruct EQ' as [? [? ?]]. subst.
+    destruct EQ'' as [? [? ?]]. subst.
+    destruct EQ''' as [? [? ?]]. subst.
+    do 4 rep_eval relax_fuel.
+Qed.
+
+Ltac interp_to_rel SOLVER :=
+  match goal with
+  | [H : eval ?e ?C ?m ?t ?reached _ = Resolved ?V ?m0 ?t0 _ |- _] =>
+    let REL := fresh "REL" in
+    assert (REL : {| Cf e C m t ~> Rs V m0 t0 |});
+    try (apply SOLVER with (l := reached); rewrite H; eauto);
+    move H at top
+  end.
+
+Lemma Eval_well_defined_r `{time T} :
+  forall FUEL (C : @dy_ctx T) m t e l V m' t'
+    (R : match eval e C m t l FUEL with
+         | Resolved V' m'' t'' _ => V = V' /\ m' = m'' /\ t' = t''
+         | _ => False
+         end),
+    {| (Cf e C m t) ~> (Rs V m' t') |}.
+Proof.
+  rename H into ET. rename H0 into OT. rename H1 into TT.
+  induction FUEL; intros; simpl in *; try (inversion R; fail).
+  destruct e; repeat des_hyp;
+  destruct R as [? [? ?]]; subst; eauto;
+  inversion HDES; subst; eauto;
+  interp_to_rel IHFUEL; eauto;
+  interp_to_rel IHFUEL; eauto;
+  interp_to_rel IHFUEL; eauto.
+Qed.
+
+Theorem Eval_well_defined `{time T} :
+  forall l e C m t V m' t',
+    (exists FUEL, 
+      match eval e C m t l FUEL with 
+      | Resolved V' m'' t'' _ => V = V' /\ m' = m'' /\ t' = t''
+      | _ => False
+      end) <->
+    ({| (Cf e C m t) ~> (Rs V m' t') |}).
+Proof.
+  intros; split; intros RR;
+  try apply Eval_well_defined_l; eauto.
+  destruct RR as [FUEL EVAL].
+  eapply Eval_well_defined_r. eauto.
+Qed.
+
+Definition extract_reached `{time T} (interp : interpreter_state) :=
+  match interp with
+  | Pending reached
+  | Error reached
+  | Resolved _ _ _ reached => reached
+  end.
+
+(* replace a shorter expression with a longer expression,
+   which is rewritten with RR to be finished off with KILLER *)
+Ltac rep_with_rew short KILLER :=
+  match goal with
+  | [RR : _ = Pending short |- _] =>
+    replace short with (extract_reached (Pending short));
+    try reflexivity; rewrite <- RR
+  | [RR : Pending short = _ |- _] =>
+    replace short with (extract_reached (Pending short));
+    try reflexivity; rewrite RR
+  | [RR : _ = Error short |- _] =>
+    replace short with (extract_reached (Error short));
+    try reflexivity; rewrite <- RR
+  | [RR : Error short = _ |- _] =>
+    replace short with (extract_reached (Error short));
+    try reflexivity; rewrite RR
+  | [RR : _ = Resolved ?V ?m ?t short |- _] =>
+    replace short with (extract_reached (Resolved V m t short));
+    try reflexivity; rewrite <- RR
+  | [RR : Resolved ?V ?m ?t short = _ |- _] =>
+    replace short with (extract_reached (Resolved V m t short));
+    try reflexivity; rewrite RR
+  | [RR : _ = short |- _] =>
+    rewrite <- RR
+  | [RR : short = _ |- _] =>
+    rewrite RR
+  end;
+  match goal with
+  | _ => apply KILLER; try right; simpl; eauto
+  end.
+
+Lemma reach_myself `{time T} :
+  forall FUEL e (C : @dy_ctx T) m t l cf,
+    In cf (Cf e C m t :: l) -> In cf (extract_reached (eval e C m t l FUEL)).
+Proof.
+  induction FUEL; intros; try (simpl; eauto; fail).
+  simpl. destruct e; repeat des_goal; simpl; eauto;
+  try right;
+  try rep_with_rew reached1 IHFUEL;
+  try rep_with_rew reached0 IHFUEL;
+  try rep_with_rew reached IHFUEL.
+Qed.
+
+Lemma reach_myself_eval `{time T} :
+  forall FUEL e (C : @dy_ctx T) m t l,
+  match eval e C m t l FUEL with
+  | Resolved V m' t' l' => In (Rs V m' t') l'
+  | _ => True
+  end.
+Proof.
+  induction FUEL; intros; try (simpl; eauto; fail);
+  destruct e; simpl; repeat des_goal; eauto;
+  repeat des_hyp; clarify; simpl; eauto;
+  try match goal with
+  | |- In (Rs ?V ?m' ?t') ?l' =>
+    match goal with
+    | [RR : eval ?e ?C ?m ?t ?l ?FUEL = Resolved V m' t' l' |- _] =>
+      specialize (IHFUEL e C m t l);
+      rewrite RR in IHFUEL
+    end
+  end; eauto.
+Qed.
+
+Ltac clar_eval := 
+  match goal with
+  | [H : eval ?e ?C ?m ?t ?l _ = Error _ |- 
+      context [eval ?e ?C ?m ?t ?l _]] =>
+    rep_eval relax_fuel_err; eauto
+  | [H : eval ?e ?C ?m ?t ?l _ = Resolved _ _ _ _ |-
+      context [eval ?e ?C ?m ?t ?l _]] =>
+    rep_eval relax_fuel; eauto
+  end.
+
+Lemma relax_fuel_reach `{time T} :
+  forall FUEL FUEL' (LE : FUEL <= FUEL') e (C : @dy_ctx T) m t l cf,
+    In cf (extract_reached (eval e C m t l FUEL)) ->
+    In cf (extract_reached (eval e C m t l FUEL')).
+Proof.
+  rename H into ET. rename H0 into OT. rename H1 into TT.
+  induction FUEL; intros.
+  simpl in *. apply reach_myself. eauto.
+  inversion LE; subst. assumption.
+  assert (FUEL <= m0) as HINT. { nia. }
+  destruct e; simpl in *; eauto.
+  - des_hyp; try clar_eval.
+    repeat des_goal;
+    try rep_with_rew reached2 reach_myself;
+    try rep_with_rew reached1 reach_myself;
+    try rep_with_rew reached0 IHFUEL;
+    try rep_eval idtac; eauto.
+    des_hyp; simpl; eauto.
+    des_hyp.
+    des_hyp; try clar_eval.
+    repeat des_goal;
+    try rep_with_rew reached2 reach_myself;
+    try rep_with_rew reached1 IHFUEL;
+    try rep_eval idtac; eauto.
+    des_hyp; simpl; eauto.
+    des_hyp; try clar_eval.
+    repeat des_goal;
+    try rep_with_rew reached2 IHFUEL;
+    rep_eval idtac; eauto.
+    des_hyp; try clar_eval.
+    repeat des_goal;
+    try rep_with_rew reached2 reach_myself;
+    try rep_with_rew reached1 IHFUEL;
+    try rep_eval idtac; eauto.
+    des_hyp; simpl; eauto.
+    des_hyp; try clar_eval; eauto.
+    des_hyp; try clar_eval.
+    repeat des_goal;
+    try rep_with_rew reached2 IHFUEL;
+    rep_eval idtac; eauto.
+  - des_hyp; try clar_eval.
+    repeat des_goal;
+    try rep_with_rew reached1 reach_myself;
+    try rep_with_rew reached0 IHFUEL;
+    try rep_eval idtac; eauto.
+    des_hyp; simpl; eauto.
+    des_hyp; try clar_eval.
+    repeat des_goal;
+    try rep_with_rew reached1 IHFUEL;
+    rep_eval idtac; eauto.
+  - des_hyp; try clar_eval.
+    repeat des_goal; try right;
+    try rep_with_rew reached2 reach_myself;
+    try rep_with_rew reached1 reach_myself;
+    try rep_with_rew reached0 IHFUEL;
+    try rep_eval idtac; eauto.
+    des_hyp; simpl; eauto.
+    des_hyp.
+    des_hyp; try clar_eval.
+    repeat des_goal; try right;
+    try rep_with_rew reached2 reach_myself;
+    try rep_with_rew reached1 IHFUEL;
+    try rep_eval idtac; eauto.
+    des_hyp; simpl; eauto.
+    des_hyp; try clar_eval.
+    repeat des_goal; try right;
+    try rep_with_rew reached2 IHFUEL;
+    rep_eval idtac; eauto.
+    des_hyp; try clar_eval.
+    repeat des_goal; try right;
+    try rep_with_rew reached2 reach_myself;
+    try rep_with_rew reached1 IHFUEL;
+    try rep_eval idtac; eauto.
+    des_hyp; simpl; eauto.
+    des_hyp; try clar_eval; eauto.
+    des_hyp; try clar_eval.
+    repeat des_goal; try right;
+    try rep_with_rew reached2 IHFUEL;
+    rep_eval idtac; eauto.
+Qed.
+
+Lemma reach_same `{time T} :
+  forall FUEL e (C : @dy_ctx T) m t l l'
+        (CONTAINED : forall cf, In cf l -> In cf l'),
+    match (eval e C m t l FUEL), (eval e C m t l' FUEL) with
+    | Resolved V m t reached, Resolved V' m' t' reached' => 
+      V = V' /\ m = m' /\ t = t' /\ (forall cf, In cf reached -> In cf reached')
+    | Error reached, Error reached'
+    | Pending reached, Pending reached' =>
+      forall cf, In cf reached -> In cf reached'
+    | _, _ => False
+    end.
+Proof.
+  rename H into ET. rename H0 into OT. rename H1 into TT.
+  induction FUEL; intros.
+  simpl. intros. destruct H; eauto.
+  assert ((forall cf : config T,
+            In cf (Cf e C m t :: l) ->
+            In cf (Cf e C m t :: l'))) as CONTAINED'.
+  { intros. simpl in *. destruct H; eauto. }
+  destruct e; simpl; eauto;
+  try (
+    (* trivial cases *)
+    lazymatch goal with 
+    | |- context [eval _ _ _ _ _ _] => fail
+    | _ => idtac
+    end;
+    repeat des_goal; repeat des_hyp; clarify;
+    repeat split; eauto;
+    intros cf OR; simpl in *; destruct OR; eauto);
+  match goal with
+    | |- context [eval ?e ?C ?m ?t _ _] =>
+      specialize (IHFUEL e C m t _ _ CONTAINED') as CONTAINED''
+  end;
+  repeat des_hyp; eauto;
+  destruct CONTAINED'' as [? [? [? CONTAINED'']]]; subst;
+  des_goal; repeat des_hyp; clarify;
+  match goal with
+  | |- context [eval ?e ?C ?m ?t _ _] =>
+    specialize (IHFUEL e C m t _ _ CONTAINED'') as CONTAINED'''
+  end;
+  repeat des_hyp; clarify;
+  destruct CONTAINED''' as [? [? [? CONTAINED''']]]; subst; eauto;
+  try match goal with
+  | |- context [project ?C ?s] =>
+    let PROJ := fresh "PROJ" in
+    destruct (project C s) eqn:PROJ; clarify
+  end;
+  match goal with
+  | |- context [eval ?e ?C ?m ?t _ _] =>
+    specialize (IHFUEL e C m t _ _ CONTAINED''') as CONTAINED''''
+  end;
+  repeat des_hyp; clarify;
+  destruct CONTAINED'''' as [? [? [? ?]]]; clarify;
+  rw; repeat split; ii; ss; des; eauto.
+Qed.
+
+Ltac separate_reach_tac cf IHFUEL HINT HINT' RR RR' :=
+  match goal with
+  | |- context [project ?C ?s] =>
+    let PROJ := fresh "PROJ" in
+    destruct (project C s) eqn:PROJ; clarify;
+    separate_reach_tac cf IHFUEL HINT HINT' RR RR'
+  | [H : context [match eval ?e ?C ?m ?t ?l ?n with _ => _ end] |-
+      context [match eval ?e ?C ?m ?t ?l0 ?n with _ => _ end]] =>
+    specialize (IHFUEL e C m t l cf) as HINT;
+    specialize (IHFUEL e C m t l0 cf) as HINT';
+    pose proof (reach_same n e C m t l0 l RR) as RR';
+    clear RR
+  | [H : context [match eval ?e ?C ?m ?t ?l ?n with _ => _ end] |-
+      context [match eval ?e ?C ?m ?t ?l0 ?n with _ => _ end]] =>
+    specialize (IHFUEL e C m t l cf) as HINT;
+    specialize (IHFUEL e C m t l0 cf) as HINT';
+    pose proof (reach_same n e C m t l l0 RR) as RR';
+    clear RR
+  end.
+
+Lemma separate_reach `{time T} :
+  forall FUEL e (C : @dy_ctx T) m t l cf,
+    In cf (extract_reached (eval e C m t l FUEL)) <->
+    In cf l \/ In cf (extract_reached (eval e C m t [] FUEL)).
+Proof.
+  rename H into ET. rename H0 into OT. rename H1 into TT.
+  induction FUEL; intros;
+  assert (forall cf, In cf [Cf e C m t] ->
+            In cf (Cf e C m t :: l)) as CONTAINED;
+  try (intros; simpl in *; destruct H; eauto; contradict);
+  simpl; split; intros SPLIT.
+  { destruct SPLIT; eauto. }
+  { destruct SPLIT as [?|[?|?]]; eauto. contradict. }
+  - destruct e;
+    try (
+      (* trivial cases *)
+      lazymatch goal with 
+      | |- context [eval _ _ _ _ _ _] => fail
+      | _ => idtac
+      end;
+      repeat des_hyp; simpl in *;
+      try destruct SPLIT as [?|[?|?]];
+      try destruct SPLIT as [?|?]; eauto);
+    separate_reach_tac cf IHFUEL HINT1 HINT1' CONTAINED RR;
+    des_goal; des_hyp;
+    try (destruct RR as [? [? [? RR]]]; subst; des_hyp);
+    try (rewrite HINT1 in SPLIT;
+      destruct SPLIT as [[?|?]|?]; eauto;
+      right; rewrite HINT1'; simpl; eauto);
+    separate_reach_tac cf IHFUEL HINT2 HINT2' RR RR';
+    des_hyp; try des_goal; des_hyp;
+    try (destruct RR' as [? [? [? RR']]]; subst; try des_hyp);
+    try match goal with
+    | |- context [project ?C ?s] =>
+      let PROJ := fresh "PROJ" in
+      destruct (project C s) eqn:PROJ; clarify
+    end;
+    try (rewrite HINT2 in SPLIT; destruct SPLIT as [SPLIT|?];
+      try (rewrite HINT1 in SPLIT; destruct SPLIT as [[?|?]|?]);
+      eauto;
+      rewrite HINT2'; rewrite HINT1'; simpl; eauto);
+    separate_reach_tac cf IHFUEL HINT3 HINT3' RR' RR'';
+    des_goal; des_hyp;
+    try (destruct RR'' as [? [? [? RR'']]]; subst; des_hyp);
+    try match goal with
+    | |- context [project ?C ?s] =>
+      let PROJ := fresh "PROJ" in
+      destruct (project C s) eqn:PROJ; clarify;
+      ss;
+      match type of SPLIT with
+      | _ \/ In ?cf ?l =>
+        destruct SPLIT as [SPLIT | SPLIT]
+      | _ => idtac
+      end
+    end; ss;
+    try (rewrite HINT3 in SPLIT; destruct SPLIT as [SPLIT|?];
+      try (rewrite HINT2 in SPLIT; destruct SPLIT as [SPLIT|?];
+        try (rewrite HINT1 in SPLIT; destruct SPLIT as [[?|?]|?]));
+      eauto;
+      rewrite HINT3'; rewrite HINT2'; rewrite HINT1'; simpl; eauto 7).
+    all:eauto.
+  - destruct e;
+    try (
+      (* trivial cases *)
+      lazymatch goal with 
+      | |- context [eval _ _ _ _ _ _] => fail
+      | _ => idtac
+      end;
+      repeat des_hyp; simpl in *;
+      try destruct SPLIT as [?|[?|[?|?]]];
+      try destruct SPLIT as [?|[?|?]];
+      try destruct SPLIT as [?|?]; eauto; contradict);
+    separate_reach_tac cf IHFUEL HINT1 HINT1' CONTAINED RR;
+    des_hyp; des_goal; try contradict;
+    try (destruct RR as [? [? [? RR]]]; subst; des_hyp);
+    try rewrite HINT1 in SPLIT; 
+    try destruct SPLIT as [?|[[?|?]|?]];
+    try rewrite HINT1';
+    simpl in *; eauto; try contradict;
+    try destruct ev;
+    separate_reach_tac cf IHFUEL HINT2 HINT2' RR RR';
+    des_hyp; des_goal; try contradict;
+    try (destruct RR' as [? [? [? RR']]]; subst; des_hyp);
+    try match goal with
+    | |- context [project ?C ?s] =>
+      let PROJ := fresh "PROJ" in
+      destruct (project C s) eqn:PROJ; clarify
+    end;
+    try rewrite HINT2 in SPLIT;
+    try destruct SPLIT as [?|[SPLIT|?]];
+    try rewrite HINT1 in SPLIT;
+    try destruct SPLIT as [[?|?]|?];
+    try rewrite HINT2'; try rewrite HINT1';
+    simpl in *; eauto; try contradict;
+    separate_reach_tac cf IHFUEL HINT3 HINT3' RR' RR'';
+    des_hyp; repeat des_goal; try contradict;
+    try (destruct RR'' as [? [? [? RR'']]]; subst);
+    try match goal with
+    | SPLIT : context [project ?C ?s], RR : project ?C ?s = _ |- _ =>
+      rewrite RR in SPLIT; ss;
+      try destruct SPLIT as [SPLIT | SPLIT]
+    end; ss;
+    try rewrite HINT3 in SPLIT;
+    try destruct SPLIT as [?|[SPLIT|?]];
+    try rewrite HINT2 in SPLIT;
+    try destruct SPLIT as [SPLIT|?];
+    try rewrite HINT1 in SPLIT;
+    try destruct SPLIT as [[?|?]|?];
+    try rewrite HINT3'; try rewrite HINT2'; try rewrite HINT1';
+    simpl in *; eauto 7; try contradict.
+    all:des; clarify; eauto.
+Qed.
+
+Lemma Reach_well_defined_l `{time T} :
+  forall e (C : dy_ctx T) m t cf' (R : {| (Cf e C m t) ~> cf' |}),
+    exists FUEL,
+      In cf' (extract_reached (eval e C m t [] FUEL)).
+Proof.
+  intros. remember (Cf e C m t) as cf.
+  ginduction R; intros; clarify;
+  try (exists 1; simpl; repeat des_goal; clarify; eauto; fail);
+  repeat match goal with
+  | [IH : context [Cf ?e ?C ?m ?t = _ -> _] |- _] =>
+    let FUEL := fresh "FUEL" in
+    let CONTAINED := fresh "CONTAINED" in
+    specialize (IH e C m t eq_refl);
+    destruct IH as [FUEL CONTAINED]
+  | [R : {| (Cf ?e ?C ?m ?t) ~> (Rs ?V' ?m' ?t') |} |- _] =>
+    let EVAL := fresh "EVAL" in
+    pose proof (Eval_well_defined_l e C m t V' m' t' R) as EVAL;
+    clear R
+  end;
+  match goal with
+  | |- exists n, In ?cf (extract_reached (eval ?e ?C ?m ?t _ n)) =>
+    repeat match goal with
+    | [H : forall l, exists n, 
+      match eval ?e' _ _ _ l n with _ => _ end |- _] =>
+      let FUEL := fresh "FUEL" in
+      let RR := fresh "RR" in
+      match e with
+      | e_app ?e1 ?e2 =>
+        match e' with
+        | e1 => specialize (H [Cf e C m t]); destruct H as [FUEL RR]
+        | e2 => 
+          match goal with 
+          | [_ : eval e1 _ _ _ _ _ = Resolved _ _ _ ?ll |- _] =>
+            specialize (H ll); destruct H as [FUEL RR]
+          end
+        | _ =>
+          match goal with
+          | [_ : eval e2 _ _ _ _ _ = Resolved _ _ _ ?ll |- _] =>
+            specialize (H ll); destruct H as [FUEL RR]
+          end
+        end
+      | e_link ?e1 ?e2 =>
+        match e' with
+        | e1 => specialize (H [Cf e C m t]); destruct H as [FUEL RR]
+        | e2 =>
+          match goal with
+          | [_ : eval e1 _ _ _ _ _ = Resolved _ _ _ ?ll |- _] =>
+            specialize (H ll); destruct H as [FUEL RR]
+          end
+        end
+      | m_app ?e1 ?e2 ?s =>
+        match e' with
+        | e1 => specialize (H [Cf e C m t]); destruct H as [FUEL RR]
+        | e2 => 
+          match goal with 
+          | [_ : eval e1 _ _ _ _ _ = Resolved _ _ _ ?ll |- _] =>
+            specialize (H ll); destruct H as [FUEL RR]
+          end
+        | _ =>
+          match goal with
+          | [_ : eval e2 _ _ _ _ _ = Resolved _ _ _ ?ll |- _] =>
+            specialize (H ll); destruct H as [FUEL RR]
+          end
+        end
+      end; des_hyp; try (destruct RR as [? [? ?]]; subst)
+    end
+  end;
+  match goal with
+  | [_ : eval _ _ _ _ _ ?n = Resolved _ _ _ _ |- _] =>
+    match goal with
+    | [_ : eval _ _ _ _ _ ?n0 = Resolved _ _ _ _ |- _] =>
+      lazymatch n0 with
+      | n => fail
+      | _ =>
+        match goal with
+        | [_ : eval _ _ _ _ _ ?n1 = Resolved _ _ _ _ |- _] =>
+          lazymatch n1 with
+          | n => fail
+          | n0 => fail
+          | _ => exists (S (Nat.max n (Nat.max n0 n1)))
+          end
+        | _ => exists (S (Nat.max n n0))
+        end
+      end
+    | _ => exists (S n)
+    end
+  end; simpl;
+  repeat rep_eval relax_fuel;
+  repeat rw;
+  try match goal with
+  | [RR : eval ?e ?C ?m ?t ?l ?n = Resolved ?V ?m' ?t' ?l' |- 
+    In _ (extract_reached (Resolved ?V ?m' ?t' ?l'))] =>
+    let H := fresh "H" in
+    pose proof (reach_myself_eval n e C m t l) as H;
+    rewrite RR in H; eauto
+  | |- context [match eval ?e ?C ?m ?t ?l ?n with | _ => _ end] =>
+    let H := fresh "H" in
+    assert (In (Cf e C m t) (extract_reached (eval e C m t l n))) as H;
+    try (apply reach_myself; simpl; eauto);
+    repeat des_goal; eauto; try right;
+    rep_with_rew reached1 reach_myself
+  end.
+  all:s; eauto.
+Qed.
+
+Lemma Reach_well_defined_r `{time T} :
+  forall FUEL e (C : @dy_ctx T) m t cf'
+         (R : In cf' (extract_reached (eval e C m t [] FUEL))),
+  {|(Cf e C m t) ~>* cf'|}.
+Proof.
+  induction FUEL; intros; simpl in *.
+  destruct R as [R | R]; inversion R; eauto.
+  repeat des_hyp;
+  repeat match goal with
+  | [RR : eval ?e ?C ?m ?t ?l ?n = _ |- _] =>
+    let H := fresh "H" in
+    assert (In cf' (extract_reached (eval e C m t l n))) as H;
+    try (rewrite RR; simpl; eauto);
+    rewrite separate_reach in H;
+    clear RR; simpl in *
+  | H : _ \/ _ |- _ => destruct H as [?|?]
+  | _ => clarify; try contradict; eauto
+  end;
+  repeat match goal with
+  | [H : In cf' (extract_reached (eval ?e ?C ?m ?t [] ?n)) |- _] =>
+    apply IHFUEL in H
+  | [H : eval ?e ?C ?m ?t _ _ = Resolved ?V ?m' ?t' _ |- _] =>
+    assert ({|(Cf e C m t) ~> (Rs V m' t')|});
+    try (eapply Eval_well_defined_r; rewrite H; eauto);
+    clear H
+  end; eauto.
+Qed.
+
+Theorem Reach_well_defined `{time T}:
+  forall e (C : @dy_ctx T) m t cf',
+    (exists FUEL, In cf' (extract_reached (eval e C m t [] FUEL))) <->
+    {| (Cf e C m t) ~>* cf' |}.
+Proof.
+  split; intros REACH; 
+  try (destruct REACH as [FUEL REACH]; eapply Reach_well_defined_r; eauto).
+  remember (Cf e C m t) as cf.
+  ginduction REACH; intros; subst.
+  exists 0. simpl. eauto.
+  apply Reach_well_defined_l in REACHl.
+  destruct REACHl as [FUEL IN].
+  destruct cf'; inversion REACH; subst; eauto;
+  match goal with
+  | [contra : {|(Rs _ _ _) ~> _|}|-_] => inversion contra
+  | [H : forall e C m t, Cf ?e' ?C' ?m' ?t' = Cf e C m t -> _ |- _] =>
+    let FUEL := fresh "FUEL'" in
+    let IN := fresh "IN'" in
+    specialize (H e' C' m' t' eq_refl);
+    destruct H as [FUEL IN]; move FUEL at top
+  end.
+  clear REACH REACHl REACHr cf'.
+  exists (FUEL + FUEL').
+  ginduction FUEL; intros.
+  destruct IN as [IN|IN]; clarify; eauto.
+  simpl in IN.
+  repeat des_hyp;
+  repeat match goal with
+  | H : _ \/ _ |- _ => destruct H as [?|?]
+  | _ => clarify; eauto 2
+  end;
+  try (apply relax_fuel_reach with (FUEL := FUEL'); try nia; assumption);
+  repeat match goal with
+  | H : In (Cf ?e0 ?C0 ?m0 ?t0) ?l0 |- _ =>
+    let IN := fresh "IN" in
+    match goal with
+    | RR : eval ?e ?C ?m ?t ?l ?n = _ |- _ =>
+      match type of RR with
+      | context [l0] =>
+        replace l0 with (extract_reached (eval e C m t l n)) in H;
+        try (rewrite RR; reflexivity);
+        rewrite separate_reach in H;
+        destruct H as [H | H]; 
+        simpl in H; try (destruct H; clarify)
+      end
+    end
+  end;
+  try (apply relax_fuel_reach with (FUEL := FUEL'); try nia; assumption);
+  eapply IHFUEL in IN'; eauto; simpl;
+  repeat match goal with
+  | H : eval ?e ?C ?m ?t ?l ?n = ?r |- 
+    context [eval ?e ?C ?m ?t ?l (?n + ?n0)] =>
+    let RR := fresh "RR" in
+    match type of H with
+    | context [Error] =>
+      assert (eval e C m t l (n + n0) = r) as RR;
+      first [apply relax_fuel_err with (FUEL := n); eauto; nia|
+      rewrite RR]
+    | context [Resolved] =>
+      assert (eval e C m t l (n + n0) = r) as RR;
+      first [apply relax_fuel with (FUEL := n); eauto; nia|
+      rewrite RR]
+    end
+  end; simpl; repeat des_goal; clarify; try right;
+  repeat match goal with
+  | RR : eval ?e ?C ?m ?t ?l ?n = ?r |- In cf'' ?ll =>
+    match type of RR with
+    | context [ll] =>
+      replace ll with (extract_reached (eval e C m t l n));
+      try (rewrite RR; reflexivity);
+      rewrite separate_reach;
+      first [right; assumption | left]
+    end
+  end.
+Qed.
